\tikz{ %
        
      
        \node[factor] (fr) {} ;
        \node[const, right=of fr] (nfr) {$f_{r_1}$}; %
	
	\node[latent, above=of fr] (d) {$d_1$} ; %
        \node[factor, above=of d] (fd) {} ;
        \node[const, right=of fd] (nfd) {$f_{d_1}$}; %
	
        
        \node[latent, above=of fd,xshift=-0.75cm] (ta) {$t_a$} ; %
        \node[factor, left=of ta] (fta) {} ;
        \node[const, above=of fta] (nfta) {$f_{t_a}$}; %
        
        
        
        \node[latent, left=of fta,yshift=1cm] (p1) {$p_1$} ; %
        \node[factor, left=of p1] (fp1) {} ;
        \node[const, above=of fp1] (nfp1) {$f_{p_1}$}; %
        
        \node[latent, left=of fp1] (s1) {$s_1$} ; %
        \node[factor, left=of s1] (fs1) {} ;
	\node[const, above=of fs1] (nfs1) {$f_{s_1}$}; %
     
        \node[latent, left=of fta,yshift=-1cm] (p2) {$p_2$} ; %
        \node[factor, left=of p2] (fp2) {} ;
        \node[const, above=of fp2] (nfp2) {$f_{p_2}$}; %
        
        \node[latent, left=of fp2] (s2) {$s_2$} ; %
        \node[factor, left=of s2] (fs2) {} ;
	\node[const, above=of fs2] (nfs2) {$f_{s_2}$}; %
        
            
        \node[latent, above=of fd,xshift=0.75cm] (tb) {$t_b$} ; %
        \node[factor, right=of tb] (ftb) {} ;
        \node[const, above=of ftb] (nftb) {$f_{t_b}$}; %
        
        \node[latent, right=of ftb,yshift=1cm] (p3) {$p_3$} ; %
        \node[factor, right=of p3] (fp3) {} ;
        \node[const, above=of fp3] (nfp3) {$f_{p_3}$}; %
        
        \node[latent, right=of fp3] (s3) {$s_3$} ; %
        \node[factor, right=of s3] (fs3) {} ;
	\node[const, above=of fs3] (nfs3) {$f_{s_3}$}; %
     
        \node[latent, right=of ftb,yshift=-1cm] (p4) {$p_4$} ; %
        \node[factor, right=of p4] (fp4) {} ;
        \node[const, above=of fp4] (nfp4) {$f_{p_4}$}; %
        
        \node[latent, right=of fp4] (s4) {$s_4$} ; %
        \node[factor, right=of s4] (fs4) {} ;
	\node[const, above=of fs4] (nfs4) {$f_{s_4}$}; %
     
        \edge[-] {fr} {d};
	\edge[-] {d} {fd};
	
        \edge[-] {fd} {ta};
        \edge[-] {ta} {fta};
        \edge[-] {fta} {p1};
        \edge[-] {p1} {fp1};
        \edge[-] {fp1} {s1};
        \edge[-] {s1} {fs1};
        \edge[-] {fta} {p2};
        \edge[-] {p2} {fp2};
        \edge[-] {fp2} {s2};
        \edge[-] {s2} {fs2};
        	
	\edge[-] {fd} {tb};
        \edge[-] {tb} {ftb};
        \edge[-] {ftb} {p3};
        \edge[-] {p3} {fp3};
        \edge[-] {fp3} {s3};
        \edge[-] {s3} {fs3};
        \edge[-] {ftb} {p4};
        \edge[-] {p4} {fp4};
        \edge[-] {fp4} {s4};
        \edge[-] {s4} {fs4};
        
	
	\node[const, below=of nfr,xshift=7cm,yshift=-1cm] (dfr) { $fr_1 = \mathbb{I}(d_1>0)$}; %
	\node[const, left=of dfr,xshift=-0.5cm] (dfd) {$fd_1 = \mathbb{I}(d_1=t_a - t_b)$}; %
	\node[const, left=of dfd,xshift=-0.5cm] (dft) {$ft_e = \mathbb{I}(t_e = \sum_{i \in A_e} p_i)$}; %
        \node[const, left=of dft,xshift=-0.5cm] (dfp) {$fp_i = N(p_i;s_i,\beta^2)$}; %
        \node[const, left=of dfp,xshift=-0.5cm] (dfs) {$fs_i = N(s_i;\mu_i,\sigma^2)$}; %
 
	
	%\node[const, right= of r, xshift=1.2cm ,yshift=-2.1cm] (result-dist) {$r_{ab} \sim B\left(\Phi\left(\frac{\mu_a - \mu_b}{\sqrt{\beta_a^2+\beta_b^2}}\right)\right)$} ; %
	      
        }